Saved work

src/dvspec/dvc3.dfy
@@ -1,6 +1,7 @@
 type ValidatorIndex = nat
-type Epoch(==)
-type Slot(==)
+type Epoch = nat 
+type Slot = nat
+const SLOTS_PER_EPOCH := 32
 type CommitteeIndex
 // type Attestation 
 type BLSSignature(==)
@@ -13,6 +14,8 @@ datatype Checkpoint = Checkpoint(
     epoch: Epoch,
     root: Root
 )
+
+type Domain(==)
 // type AttestationDuty 
 datatype AttestationData = AttestationData(
     slot: Slot,
@@ -24,7 +27,17 @@ datatype AttestationData = AttestationData(
     target: Checkpoint
 )
 // type ProposerDuty
-type BeaconBlock(==)
+datatype BeaconBlock = BeaconBlock(
+    body: BeaconBlockBody
+    // ... Other fields irrelevant to this spec
+)
+
+datatype BeaconBlockBody = BeaconBlockBody(
+    attestations: seq<Attestation>,
+    state_root: Root
+    // ... Other fields irrelevant to this spec
+)
+
 type SyncCommitteeDuty   
 type Version
 
@@ -86,12 +99,97 @@ datatype Optional<T> = Some(v: T) | None
 function method consensus_on_attestation(slashing_db: AttestationSlashingDB, attestation_duty: AttestationDuty): AttestationData
 
 function method compute_start_slot_at_epoch(epoch: Epoch): Slot
+{
+    epoch * SLOTS_PER_EPOCH
+}
 
 function method bn_get_fork_version(slot: Slot): Version
 
-function method compute_attestation_signing_root(attestation_data: AttestationData): Root
 
-function method rs_sign_attestation(attestation_data: AttestationData, fork_version: Version, signing_root: Root): BLSSignature
+// https://ethereum.github.io/beacon-APIs/#/Beacon/getStateValidator
+function method bn_get_validator_index(
+    state_id: Root,
+    validator_id: BLSPubkey
+): Optional<ValidatorIndex>
+
+// https://ethereum.github.io/beacon-APIs/?urls.primaryName=v1#/Beacon/getEpochCommittees
+function method bn_get_epoch_committees(
+    state_id: Root,
+    index: CommitteeIndex
+): seq<ValidatorIndex>
+
+datatype DomainTypes = 
+    | DOMAIN_BEACON_ATTESTER
+
+
+// TDOO: What about the genesis_validator_root parameter?
+function method compute_domain(
+    domain_type: DomainTypes,
+    fork_version: Version
+): (domain: Domain)
+
+
+lemma compute_domain_properties()
+ensures forall d1, f1, d2, f2 :: compute_domain(d1, f2) == compute_domain(d2, f2) ==>
+    && d1 == d2 
+    && f1 == f2
+
+function method compute_signing_root<T>(
+    data: T,
+    domain: Domain
+): Root
+
+lemma compute_signing_root_properties<T>()
+ensures forall da1, do1, da2, do2 ::
+    compute_signing_root<T>(da1, do1) == compute_signing_root<T>(da2, do2) ==>
+        && da1 == da2 
+        && do1 == do2
+
+// TODO: Fix Python code to match the following (Python code uses epoch)
+function method compute_attestation_signing_root(attestation_data: AttestationData, fork_version: Version): Root
+{
+    var domain := compute_domain(DOMAIN_BEACON_ATTESTER, fork_version);
+    compute_signing_root(attestation_data, domain)
+}
+
+function method rs_sign_attestation(
+    attestation_data: AttestationData, 
+    fork_version: Version, 
+    signing_root: Root,
+    pubkey: BLSPubkey
+): BLSSignature
+requires signing_root == compute_attestation_signing_root(attestation_data, fork_version)
+
+lemma rs_attestation_sign_and_verification_propetries<T>()
+ensures forall attestation_data, fork_version, signing_root, pubkey |
+    rs_sign_attestation.requires(attestation_data, fork_version, signing_root, pubkey) ::
+    verify_bls_siganture(
+        signing_root,
+        rs_sign_attestation(attestation_data, fork_version, signing_root, pubkey),
+        pubkey
+    )
+ensures forall signing_root, signature, pubkey ::
+    verify_bls_siganture(signing_root, signature, pubkey) <==>
+        exists attestation_data, fork_version ::
+        && rs_sign_attestation.requires(attestation_data, fork_version, signing_root, pubkey)
+        && signature == rs_sign_attestation(attestation_data, fork_version, signing_root, pubkey)
+
+ensures forall ad1, fv1, sr1, pk1, ad2, fv2, sr2, pk2 ::
+            && rs_sign_attestation.requires(ad1, fv1, sr1, pk1)
+            && rs_sign_attestation.requires(ad2, fv2, sr2, pk2)
+            && rs_sign_attestation(ad1, fv1, sr1, pk1) == rs_sign_attestation(ad2, fv2, sr2, pk2) 
+            ==>
+            && sr1 == sr2 
+            && pk1 == pk2
+
+
+predicate verify_bls_siganture<T>(
+    data: T,
+    signature: BLSSignature,
+    pubkey: BLSPubkey
+)
+
+        
 
 method update_attestation_slashing_db(slashing_db: AttestationSlashingDB, attestation_data: AttestationData, attestation_duty_pubkey: BLSPubkey)
 
@@ -101,27 +199,27 @@ function f_update_attestation_slashing_db(slashing_db: AttestationSlashingDB, at
 method broadcast_attestation_signature_share(attstationg: AttestationShare)
 
 
-method serve_attestation_duty(slashing_db: AttestationSlashingDB, attestation_duty: AttestationDuty)
-{
-    // TODO: Is lock on consensus the best way to do this? Does lock on slashing DB work?
-    // Obtain lock on consensus_on_attestation here.
-    // Only a single consensus_on_attestation instance should be
-    // running at any given time
-    var attestation_data := consensus_on_attestation(slashing_db, attestation_duty);
-    // assert consensus_is_valid_attestation_data(slashing_db, attestation_data, attestation_duty)
-    // Release lock on consensus_on_attestation here.
-    // Add attestation to slashing DB
-    update_attestation_slashing_db(slashing_db, attestation_data, attestation_duty.pubkey);
-    // Sign attestation using RS
-    // TODO: Reuse fork version from here in compute_domain
-    var fork_version := bn_get_fork_version(compute_start_slot_at_epoch(attestation_data.target.epoch));
-    var attestation_signing_root := compute_attestation_signing_root(attestation_data);
-    var attestation_signature_share := rs_sign_attestation(attestation_data, fork_version, attestation_signing_root);
-    // TODO: What is attestation_signature_share.aggregation_bits?
-    var attestation_with_signature_share := AttestationShare(data :=attestation_data, signature :=attestation_signature_share);
-    // TODO: Should we just gossip & recombine the signature shares without attestation data?
-    broadcast_attestation_signature_share(attestation_with_signature_share);
-}
+// method serve_attestation_duty(slashing_db: AttestationSlashingDB, attestation_duty: AttestationDuty)
+// {
+//     // TODO: Is lock on consensus the best way to do this? Does lock on slashing DB work?
+//     // Obtain lock on consensus_on_attestation here.
+//     // Only a single consensus_on_attestation instance should be
+//     // running at any given time
+//     var attestation_data := consensus_on_attestation(slashing_db, attestation_duty);
+//     // assert consensus_is_valid_attestation_data(slashing_db, attestation_data, attestation_duty)
+//     // Release lock on consensus_on_attestation here.
+//     // Add attestation to slashing DB
+//     update_attestation_slashing_db(slashing_db, attestation_data, attestation_duty.pubkey);
+//     // Sign attestation using RS
+//     // TODO: Reuse fork version from here in compute_domain
+//     var fork_version := bn_get_fork_version(compute_start_slot_at_epoch(attestation_data.target.epoch));
+//     var attestation_signing_root := compute_attestation_signing_root(attestation_data, fork_version);
+//     var attestation_signature_share := rs_sign_attestation(attestation_data, fork_version, attestation_signing_root);
+//     // TODO: What is attestation_signature_share.aggregation_bits?
+//     var attestation_with_signature_share := AttestationShare(data :=attestation_data, signature :=attestation_signature_share);
+//     // TODO: Should we just gossip & recombine the signature shares without attestation data?
+//     broadcast_attestation_signature_share(attestation_with_signature_share);
+// }
 
 
 
@@ -135,31 +233,33 @@ datatype ProcessOutput<!T1, T2> =
         // ,initial_value: T1
         // ,validity_function: T1 -> bool
     )
-// |   StopConsensus(
-//         start_consensus_with_instance_id: (CONSENSUS_TYPE, Slot)
-//     )
+|   StopConsensus(
+        stop_consensus_with_instance_id: set<Slot>
+    )
 |   SignatureShareToBroadcastAndNewProcessState(signature_share: T2, new_process_state: ServeAttesationProcess)
 |   NewProcessState(new_process_state: ServeAttesationProcess)
 |   NewProcessStateAndAggregatedAttestation(
         aggregated_attestations: set<Attestation>,
         new_process_state: ServeAttesationProcess
 )
+|   SendAggregatedAttestation(
+        aggregated_attestation: Attestation
+)
+|   NoChangeNothingToDo
 
 type COValidatorID(==)
 
 datatype ServeAttesationProcess = ServeAttesationProcess(
     attestation_duty: AttestationDuty,
-    construct_signed_attestation_signature: (AttestationData, set<BLSSignature>) -> Optional<BLSSignature>,
-    signature_shares_db: AttestationSignatureShareDB,
+    construct_signed_attestation_signature: (set<AttestationShare>) -> Optional<BLSSignature>,
+    attestation_shares_db: AttestationSignatureShareDB,
     // co_validators: map<BLSPubkey, COValidatorID>
-    slashing_db: AttestationSlashingDB
+    slashing_db: AttestationSlashingDB,
+    dv_pubkey: BLSPubkey,
+    co_validator_pubkey: BLSPubkey,
+    all_aggregated_attestations: set<Attestation>
 )
 
-predicate verify_bls_siganture<T>(
-    data: T,
-    signature: BLSSignature,
-    pubkey: BLSPubkey
-)
 
 datatype ServeAttestationProcessInputEvent = 
 | StartProcess(slashing_db: AttestationSlashingDB)
@@ -208,8 +308,8 @@ function f_serve_attestation_duty_consensus_finished(
     // Sign attestation using RS
     // TODO: Reuse fork version from here in compute_domain
     var fork_version := bn_get_fork_version(compute_start_slot_at_epoch(decided_attestation_data.target.epoch));
-    var attestation_signing_root := compute_attestation_signing_root(decided_attestation_data);
-    var attestation_signature_share := rs_sign_attestation(decided_attestation_data, fork_version, attestation_signing_root);
+    var attestation_signing_root := compute_attestation_signing_root(decided_attestation_data, fork_version);
+    var attestation_signature_share := rs_sign_attestation(decided_attestation_data, fork_version, attestation_signing_root, process.co_validator_pubkey);
     // TODO: What is attestation_signature_share.aggregation_bits?
     var attestation_with_signature_share := AttestationShare(data := decided_attestation_data, signature :=attestation_signature_share);
     // TODO: Should we just gossip & recombine the signature shares without attestation data?
@@ -220,7 +320,7 @@ function f_serve_attestation_duty_consensus_finished(
     )
 }
 
-type AttestationSignatureShareDB = map<AttestationData, set<BLSSignature>>
+type AttestationSignatureShareDB = map<AttestationData, set<AttestationShare>>
 
 // function mapPutIfAbsent<T1,T2>(M:map<T1,T2>, key:T1, value:T2): map<T1,T2>
 //     {
@@ -241,8 +341,11 @@ function getOrDefault<T1,T2>(M:map<T1,T2>, key:T1, default:T2): T2
     }   
 
 function get_aggregation_bits(
-    process: ServeAttesationProcess
+    index: nat
 ): seq<bool>
+{
+    seq(index, i => if i + 1 == index then true else false)
+}
 
 datatype AggregatedAttestationAndAttestationSignatureShareDB = AggregatedAttestationAndAttestationSignatureShareDB(
     aggregated_attestations: set<Attestation>,
@@ -266,34 +369,81 @@ function construct_signed_attestation_signature(
 
 function f_listen_for_attestation_signature_shares(
     process: ServeAttesationProcess, 
-    // signature_shares_db: AttestationSignatureShareDB, 
+    // attestation_shares_db: AttestationSignatureShareDB, 
     attestation_share: AttestationShare): ProcessOutput<AttestationData, AttestationShare>
 {
 
-    var sets_of_signatures_for_attestation_data := getOrDefault(process.signature_shares_db, attestation_share.data, {});
+    var sets_of_signatures_for_attestation_data := getOrDefault(process.attestation_shares_db, attestation_share.data, {});
 
-    var new_signature_shares_db := process.signature_shares_db[attestation_share.data := 
-        sets_of_signatures_for_attestation_data + {attestation_share.signature}];
+    var new_attestation_shares_db := process.attestation_shares_db[attestation_share.data := 
+        sets_of_signatures_for_attestation_data + {attestation_share}];
 
     var aggregated_attestations := 
         set k | 
-                && k in new_signature_shares_db.Keys 
-                && process.construct_signed_attestation_signature(k, new_signature_shares_db[k]).isPresent()
+                && k in new_attestation_shares_db.Keys 
+                && process.construct_signed_attestation_signature(new_attestation_shares_db[k]).isPresent()
             ::
                 Attestation(
-                    aggregation_bits := get_aggregation_bits(process),
+                    aggregation_bits := get_aggregation_bits(process.attestation_duty.validator_index),
                     data := k,
-                    signature := process.construct_signed_attestation_signature(k, new_signature_shares_db[k]).get()
+                    signature := process.construct_signed_attestation_signature(new_attestation_shares_db[k]).get()
                 );
                 
+    var all_aggregated_attestations := 
+        process.all_aggregated_attestations + aggregated_attestations;
 
     NewProcessStateAndAggregatedAttestation(
         aggregated_attestations,
-        new_process_state := process.(signature_shares_db := new_signature_shares_db)
+        new_process_state := process.(
+            attestation_shares_db := new_attestation_shares_db,
+            all_aggregated_attestations := all_aggregated_attestations
+        )
     )
 }
 
+function f_listen_for_new_imported_blocks(
+    process: ServeAttesationProcess, 
+    block: BeaconBlock
+): ProcessOutput<AttestationData, AttestationShare>
+{
+    var valIndex := bn_get_validator_index(block.body.state_root, process.dv_pubkey);
+    
+    var s := set a |
+            && a in block.body.attestations
+            // && a.data.slot == process.attestation_duty.slot 
+            // && a.data.index == process.attestation_duty.committee_index
+            && var committee := bn_get_epoch_committees(block.body.state_root, a.data.index);
+            && valIndex.Some?
+            && valIndex.v in committee
+            && var i:nat :| i < |committee| && committee[i] == valIndex.v;
+            && i < |a.aggregation_bits|
+            && a.aggregation_bits[i]
+        ::
+            a.data.slot;
+    
+    StopConsensus(s)
+}
+
+function f_resend_attestation_share(
+    process: ServeAttesationProcess
+): ProcessOutput<AttestationData, AttestationShare>
+{
+    var aggregated_attestations_to_send :=
+        set a |
+            &&  a in process.all_aggregated_attestations
+            && a.data.slot == process.attestation_duty.slot;
+
+    if |aggregated_attestations_to_send| > 0 then
+        var aggregated_attestation :| aggregated_attestation in aggregated_attestations_to_send;
+        SendAggregatedAttestation(
+            aggregated_attestation
+        )
+    else
+        NoChangeNothingToDo
+}
+
 type NodeID(==)
+
 datatype NSState = NSState
 
 /*
@@ -341,7 +491,7 @@ datatype DSVState = DSVState(
     slashing_dbs_used_for_validating_attestations: imaptotal<Slot, set<AttestationSlashingDB>>,
     aggregated_attestations_sent: set<Attestation>,
     attestation_duties_served: map<AttestationDuty, set<BLSPubkey>>,
-    construct_signed_attestation_signature: (AttestationData, set<BLSSignature>) -> Optional<BLSSignature>
+    construct_signed_attestation_signature: (set<AttestationShare>) -> Optional<BLSSignature>
 )
 
 function f(n:nat): nat
@@ -364,31 +514,39 @@ predicate DSVInit(
     && |s.adversary.nodes| <= f(|s.all_nodes|)
     && (
         forall 
-            data: AttestationData, 
-            sig_shares: set<BLSSignature> 
+            att_shares: set<AttestationShare>
             ::
             (
-                exists verifiable_sig_shares: set<BLSSignature> ::
-                    && verifiable_sig_shares <= sig_shares
-                    && quorum(|verifiable_sig_shares|) >= |s.all_nodes|
-                    && (forall sig_share |
-                        sig_share in verifiable_sig_shares ::
-                            exists signer :: 
+                && exists verifiable_att_shares: set<AttestationShare>, data: AttestationData, fork_version: Version ::
+                    && verifiable_att_shares <= att_shares
+                    && var signing_root := compute_attestation_signing_root(data, fork_version);
+                    && |verifiable_att_shares| >= quorum(|s.all_nodes|)
+                    && (forall att_share |
+                            att_share in verifiable_att_shares ::
+                            && att_share.data == data 
+                            && exists signer :: 
                                 && signer in s.all_nodes
-                                && verify_bls_siganture(data, sig_share, signer)
+                                && verify_bls_siganture(signing_root, att_share.signature, signer)
                     )
             )
             <==>
-                s.construct_signed_attestation_signature(data, sig_shares).isPresent()
+                s.construct_signed_attestation_signature(att_shares).isPresent()
     )    
     &&
         (
         forall 
-            data: AttestationData, 
-            sig_shares: set<BLSSignature> 
+            att_shares: set<AttestationShare>
             ::
-                var constructed_sig := s.construct_signed_attestation_signature(data, sig_shares);
-                constructed_sig.isPresent() ==> verify_bls_siganture(data, constructed_sig.get(), s.dv_pubkey)
+                var constructed_sig := s.construct_signed_attestation_signature(att_shares);
+                constructed_sig.isPresent() ==>  
+                    forall verifiable_att_shares: set<AttestationShare>, data: AttestationData, fork_version: Version |
+                        && verifiable_att_shares <= att_shares
+                        && |verifiable_att_shares| >= quorum(|s.all_nodes|)
+                        && (forall att_share |
+                                att_share in verifiable_att_shares :: att_share.data == data)
+                        ::
+                                && var signing_root := compute_attestation_signing_root(data, fork_version);
+                                verify_bls_siganture(signing_root, constructed_sig.get(), s.dv_pubkey)
 
     )   
     && s.attestations_shares_sent == {}
@@ -398,13 +556,17 @@ predicate DSVInit(
     && s.attestation_duties_served == map[]
     && no_slashing_conditions_in_the_slashing_db(initial_slashing_db)    
     && (
-        forall p | p in s.honest_nodes_states.Values ::
-            p == ServeAttesationProcess(
-                attestation_duty := p.attestation_duty,
-                construct_signed_attestation_signature := s.construct_signed_attestation_signature,
-                slashing_db := initial_slashing_db,
-                signature_shares_db := map[]
-            )
+        forall n | n in s.honest_nodes_states.Keys ::
+            s.honest_nodes_states[n] ==
+                ServeAttesationProcess(
+                    attestation_duty := s.honest_nodes_states[n].attestation_duty,
+                    construct_signed_attestation_signature := s.construct_signed_attestation_signature,
+                    slashing_db := initial_slashing_db,
+                    attestation_shares_db := map[],
+                    dv_pubkey := s.dv_pubkey,
+                    co_validator_pubkey := n,
+                    all_aggregated_attestations := {}
+                )
     )
 }
 
@@ -416,6 +578,8 @@ predicate DSVNext(
     slashing_db_used_to_check_attestation_data: AttestationSlashingDB,
     attestation_signature_share_received: AttestationShare,
     attestation_duty_to_be_served: AttestationDuty,
+    newBlock: BeaconBlock,
+    aggregated_attestations_to_be_sent: set<Attestation>,
     s': DSVState
 )
 {
@@ -437,9 +601,8 @@ predicate DSVNext(
                         s.honest_nodes_states[node_taking_step],
                         attestation_duty_to_be_served
                     );
-                    && s'.attestation_duties_served.Keys == s.attestation_duties_served.Keys + {attestation_duty_to_be_served}
-                    && var s_attestation_duty_to_be_served := getOrDefault(s.attestation_duties_served, attestation_duty_to_be_served, {}); 
-                    && s'.attestation_duties_served[attestation_duty_to_be_served] == s_attestation_duty_to_be_served + {node_taking_step}
+                    && s'.attestation_duties_served.Keys == s.attestation_duties_served.Keys + {attestation_duty_to_be_served} 
+                    && s'.attestation_duties_served[attestation_duty_to_be_served] == getOrDefault(s.attestation_duties_served, attestation_duty_to_be_served, {}) + {node_taking_step}
                     && var consensus_id := process_output.start_consensus_with_instance_id;
                     && s'.consensus_on_attestation_data == s.consensus_on_attestation_data[consensus_id := s'.consensus_on_attestation_data[consensus_id]]
                     && s'.consensus_on_attestation_data[consensus_id].honest_nodes_running == s.consensus_on_attestation_data[consensus_id].honest_nodes_running + {node_taking_step}
@@ -460,6 +623,7 @@ predicate DSVNext(
                         || (
                             && s.consensus_on_attestation_data[attestation_consensus_instance].decided_value.isPresent()
                             && s.consensus_on_attestation_data[attestation_consensus_instance].decided_value.get() == decided_attestation_data
+                            && s'.consensus_on_attestation_data[attestation_consensus_instance].decided_value == s.consensus_on_attestation_data[attestation_consensus_instance].decided_value
                         )
                         || (
                             && !s.consensus_on_attestation_data[attestation_consensus_instance].decided_value.isPresent()
@@ -490,16 +654,45 @@ predicate DSVNext(
                     );
                     && s'.honest_nodes_states[node_taking_step] == process_output.new_process_state
                     && s'.aggregated_attestations_sent == s.aggregated_attestations_sent + process_output.aggregated_attestations
+                    && aggregated_attestations_to_be_sent == process_output.aggregated_attestations
                     && s' == s.(
                         honest_nodes_states := s'.honest_nodes_states,
                         aggregated_attestations_sent := s'.aggregated_attestations_sent,
                         slashing_dbs_used_for_validating_attestations := s'.slashing_dbs_used_for_validating_attestations                     
                     )
                 )
+                ||  (
+
+                    && var process_output := f_listen_for_new_imported_blocks(
+                        s.honest_nodes_states[node_taking_step],
+                        newBlock
+                    );
+                    && forall cInstnace | cInstnace in s.consensus_on_attestation_data ::
+                        if cInstnace in process_output.stop_consensus_with_instance_id then
+                            && s'.consensus_on_attestation_data[cInstnace].honest_nodes_running == s.consensus_on_attestation_data[cInstnace].honest_nodes_running - {node_taking_step}
+                            && s'.consensus_on_attestation_data[cInstnace] == s.consensus_on_attestation_data[cInstnace].(
+                                honest_nodes_running := s'.consensus_on_attestation_data[cInstnace].honest_nodes_running
+                            )
+                        else
+                            s'.consensus_on_attestation_data[cInstnace] == s.consensus_on_attestation_data[cInstnace]
+                    && s' == s.(
+                        consensus_on_attestation_data := s'.consensus_on_attestation_data
+                    )
+                )
+                || (
+                    && var process_output := f_resend_attestation_share(
+                        s.honest_nodes_states[node_taking_step]
+                    );
+                    &&  s' == s
+                    &&
+                        if process_output.NoChangeNothingToDo? then
+                            aggregated_attestations_to_be_sent == {}
+                        else 
+                            aggregated_attestations_to_be_sent == {process_output.aggregated_attestation}
+                )
             )
             && (
-                forall consensus_id
-                    ::
+                forall consensus_id: Slot ::
                     s'.slashing_dbs_used_for_validating_attestations[consensus_id] == s.slashing_dbs_used_for_validating_attestations[consensus_id] +
                         if node_taking_step in s'.consensus_on_attestation_data[consensus_id].honest_nodes_running then
                             {s'.honest_nodes_states[node_taking_step].slashing_db}
@@ -521,8 +714,8 @@ predicate DSVNext(
             && (forall aggregated_attestation_sent | aggregated_attestation_sent in new_aggregated_attestations_sent ::
                     exists attestation_shares ::
                             && attestation_shares <= s'.attestations_shares_sent
-                            && var sig_shares := set x | x in attestation_shares :: x.signature;
-                            && var constructed_sig := s.construct_signed_attestation_signature(aggregated_attestation_sent.data, sig_shares);
+                            // && var sig_shares := set x | x in attestation_shares :: x.signature;
+                            && var constructed_sig := s.construct_signed_attestation_signature(attestation_shares);
                             && constructed_sig.isPresent()
                             && constructed_sig.get() == aggregated_attestation_sent.signature
             )
